
\preClass{Inverting Laplace Transforms}

\begin{problem}
\item Use a table to determine the following Laplace transforms:

  \begin{subproblem}
  \item 
    \begin{eqnarray*}
      \laplace{e^{-5t}}
    \end{eqnarray*}
    \vfill

  \item 
    \begin{eqnarray*}
      \laplace{t^4-3t^2}
    \end{eqnarray*}
    \vfill
      
  \item 
    \begin{eqnarray*}
      \laplace{4te^{-5t} + t\cos(2t) - t^2e^{3t}}
    \end{eqnarray*}
    \vfill

  \end{subproblem}
\end{problem}

\actTitle{Solving Differential Equations with the Laplace Transform}
\begin{problem}
\item Express the Laplace transform of $y'$ in terms of $\laplace{y}$.
  \begin{subproblem}
    \item Use integration by parts to express the following integral
      in terms of an integral that has $y$ in it rather than $y'$:
      \begin{eqnarray*}
        \laplace{y'} & = & \int^\infty_0 y' e^{-st} ~ dt.
      \end{eqnarray*}
      \vfill

    \item Simplify the express to show that $\laplace{y'} = -y(0) + s\laplace{y}$.
      \vfill

  \end{subproblem}


  \clearpage

\item Determine expressions for the Laplace transforms of the
  solutions to each of the following differential equations. (Do not
  solve for the solution to the differential equation just determine
  the value of $\laplace{y}$.)

  \begin{subproblem}
  \item 
    \begin{eqnarray*}
      y' + y & = & 0, \\
      y(0) & = & 2.
    \end{eqnarray*}
    \vfill

  \item 
    \begin{eqnarray*}
      y' + 2y & = & e^{-2t}, \\
      y(0) & = & -3.
    \end{eqnarray*}
    \vfill

  \item 
    \begin{eqnarray*}
      y'' + 4y & = & t + 3e^{-t}, \\
      y(0) & = & 0, \\
      y'(0) & = & 3.
    \end{eqnarray*}
    \vfill

  \item 
    \begin{eqnarray*}
      y'' + 6y' + 10 & = & -3t + 2e^{5t}, \\
      y(0) & = & 0, \\
      y'(0) & = & 2.
    \end{eqnarray*}
    \vfill


  \end{subproblem}


\end{problem}


\actTitle{Laplace Transforms}
\begin{problem}

\item Solve for the solution of the differential equation for each of
  the differential equations.

  \begin{subproblem}
  \item 
    \begin{eqnarray*}
      y' + y & = & 0, \\
      y(0) & = & 2.
    \end{eqnarray*}
    \vfill

  \item 
    \begin{eqnarray*}
      y' + 2y & = & e^{-2t}, \\
      y(0) & = & -3.
    \end{eqnarray*}
    \vfill

    \clearpage

  \item 
    \begin{eqnarray*}
      y'' + 4y & = & t + 3e^{-t}, \\
      y(0) & = & 0, \\
      y'(0) & = & 3.
    \end{eqnarray*}
    \vfill

  \item 
    \begin{eqnarray*}
      y'' + 6y' + 10 & = & -3t + 2e^{5t}, \\
      y(0) & = & 0, \\
      y'(0) & = & 2.
    \end{eqnarray*}
    \vfill


  \end{subproblem}


\end{problem}

