  \actTitle{Separable ODEs}
  \begin{problem}
  \item Expand each expression using partial fractions:
    \begin{subproblem}
    \item $\frac{y}{y^2-4}$
      \vfill

    \item $\frac{4}{y^2-2y}$.
      \vfill
      
    \item $\frac{3}{y^2-3y+2}$
      \vfill

    \end{subproblem}
    \clearpage
  \item Find the solutions to the following ODEs. 
    \begin{subproblem}
    \item $y' = y^2 + 1$, $y(0)=3$.
      \vfill
    \item $y' = yt - t$, $y(0)=4$.
      \vfill
    \item $y'=y(y-1)$, $y(0)=5$.
      \vfill
    \item $y' = y^2(y+1)$, $y(0)=10$.
      \vfill
    \end{subproblem}

  \end{problem}


  \actTitle{Linear Differential Equations}
  For each problem below $C_1$ and $C_2$ are constants.
  \begin{problem}

  \item Show that $y=C_1 e^{3t}-\frac{1}{3}$ is a solution to the
    differential equation $y'=3y+1$.
    \vfill

  \item Show that $y=C_1 e^{t} + C_2 e^{-2t}$ is a solution to the
    differential equation $y''+3y'+2y=0$.

    \vfill

    \clearpage

  \item Suppose that you have the following differential equation:
    \begin{eqnarray*}
      \frac{d}{dt} \left( y(t) e^{3t} \right) & = & e^{3t}.
    \end{eqnarray*}
    Take the antiderivative of each side and express the result
    without any derivatives. (Do not forget the constant of
    integration.)  
    
    \vfill

  \item Simplify the expression and solve for $y(t)$. 
    \vfill

    \clearpage

  \item Suppose that $y$ is a function of $t$. Use the product rule to
    find the derivative of the function $\left(y(t) e^{3t}\right)$.
    \vfill

  \item Suppose that the expression in the previous problem is equal
    to $e^{3t}$.  Set the previous expression equal to $e^{3t}$ and
    simplify. What is the new differential equation?
    \vfill

  \item What is the solution to the differential equation?

\end{problem}

