
\title{Ordinary Differential Equations}
\subtitle{Math 232 - Week 2, Day 2}

\author{Kelly Black}
\institute{Clarkson University}
\date{7 Sep 2011}

\begin{frame}
  \titlepage
\end{frame}

\begin{frame}
  \frametitle{Outline}
  \tableofcontents[pausesection,hideallsubsections]
\end{frame}


\section{First Order Linear Equations}


\begin{frame}
  \frametitle{Another ``Special Form''}

  \begin{eqnarray*}
    y' + p(t) y & = & f(t)
  \end{eqnarray*}

  read pages 63-66 

  I will only cover integrating factors in class.

\end{frame}

\section{Product Rule}

\begin{frame}
  \frametitle{The Product Rule}

  \begin{eqnarray*}
    \frac{d}{dt} \lp u v \rp & = & u' v + u v'
  \end{eqnarray*}

\end{frame}


\begin{frame}
  \frametitle{Example}

  \begin{eqnarray*}
    y ' & = & - y + t \\
    \uncover<2->{ y' + y & = & t} \\
    \uncover<3->{y' e^t + y e^ t & = & t e^t } \\
    \uncover<4->{\deriv{~}{t} \lp y e^t \rp & = & t e^t } \\
    \uncover<5->{y e^t  & = & \int t e^t ~ dt } \\
    \uncover<6->{y e^t  & = & t e^t - e^t + C } \\
    \uncover<7->{ y & = & t -1 + Ce^{-t}}
  \end{eqnarray*}

  \uncover<8->{How did I know how to do this?}


\end{frame}


\section{Integrating Factors}

\begin{frame}
  \frametitle{Let's Backup}

  \begin{eqnarray*}
    y' + p(t) y & = & f(t) \\
    e^{G(t)} y' + p(t) e^{G(t)} y & = & e^{G(t)} f(t)
  \end{eqnarray*}


\end{frame}



\begin{frame}
  \frametitle{Product Rule Redux}

  \begin{eqnarray*}
    \frac{d}{dt} \lp e^{G(t)} \rp & = & G'(t) e^{G(t)} 
  \end{eqnarray*}

  Let
  \begin{eqnarray*}
    G'(t) & = & p(t) \\
    \Rightarrow G(t) & = & \int p(t) ~ dt.
  \end{eqnarray*}


\end{frame}


\begin{frame}
  \frametitle{Product Rule Redux}

  \begin{eqnarray*}
    \frac{d}{dt} \lp e^{G(t)} y \rp & = & e^{G(t)} y' + G'(t) e^{G(t)} y \\
    & = & e^{G(t)} y' + p(t) e^{G(t)} y \\
    & = & e^{G(t)} \lp y' + p(t) y \rp \\
    & = & f(t) e^{G(t)}
  \end{eqnarray*}

  or
  \begin{eqnarray*}
    e^{G(t)} y & = & \int f(t) e^{G(t)} ~ dt
  \end{eqnarray*}
  \textit{Hope and pray!}

\end{frame}


\section{Examples}

\begin{frame}
  \frametitle{Example}

  \vspace*{-3em}
  \begin{eqnarray*}
    y' + 2y & = & t \\
    p(t) & = & 2, \\
    \int 2 ~ dt & = & 2t + K, \\
    e^{2t} & & 
  \end{eqnarray*}

  \begin{eqnarray*}
    e^{2t} y' + 2 e^{2t} y & = & t e^{2t}, \\
    \frac{d}{dt} \lp e^{2t} y \rp & = & t e^{2t} \\
    e^{2t} y & = & \int t e^{2t} ~ dt \\
    e^{2t} y & = & \half t e^{2t} - \frac{1}{4} e^{2t} + C \\
    y & = & \half t - \frac{1}{4} + C e^{-2t}
  \end{eqnarray*}

\end{frame}



\begin{frame}
  \frametitle{Example}

  \vspace*{-3em}
  \begin{eqnarray*}
    y' & = & ty + t^3 \\
    y' - ty & = & t^3 \\
    p(t) & = & -t, \\
    \int -t ~ dt & = & -\half t^2 + K \\
    e^{-\half t^2} & & 
  \end{eqnarray*}

  \begin{eqnarray*}
    y' e^{-\half t^2} - t e^{-\half t^2} y & = & t^3 e^{-\half t^2} \\
    \frac{d}{dt} \lp y e^{-\half t^2} \rp & = & \int t^3 e^{-\half t^2} ~ dt \\
    y e^{-\half t^2} & = & -t^2 e^{-\half t^2} - 2 e^{-\half t^2} + C \\
    y & = & -t^2 - 2 + C e^{\half t^2}
  \end{eqnarray*}

\end{frame}



\begin{frame}
  \frametitle{Example}

  \begin{eqnarray*}
    y' & = & -\frac{4}{t} y + 4 t \\
    y' + \frac{4}{t} y & = & 4 t \\
    p(t) & = & \frac{4}{t} \\
    \int \frac{4}{t} ~ dt & = & 4 \ln(t) + K \\
    e^{4 \ln(t) } & = & t^4
  \end{eqnarray*}

\end{frame}

\begin{frame}
  \frametitle{Example - continues}

  \begin{eqnarray*}
    t^4 y' + 4t^3& = & 4 t^5 \\
    \frac{d}{dt} \lp t^4 y \rp & = & 4 t^5 \\
    t^4 y & = & \int 4 t^5 ~ dt \\
    t^4 y & = & \frac{4}{6} t^6 + C \\
    y & = & \frac{2}{3} t^2 + \frac{C}{t^4}
  \end{eqnarray*}

\end{frame}



\begin{frame}
  \frametitle{Example}

  \vspace*{-3em}
  \begin{eqnarray*}
    y' & = & -\frac{1}{t} y + \frac{1}{t^2 -1} \\
    y' + \frac{1}{t} y & = & \frac{1}{t^2 -1} \\
    p(t) & = & \frac{1}{t} \\
    \int \frac{1}{t} ~ dt & = & \ln(t) + k \\
    e^{\ln(t)} & = & t
  \end{eqnarray*}

  \begin{eqnarray*}
    t y' + y & = & \frac{t}{t^2-1} \\
    \frac{d}{dt} \lp t y \rp & = & \frac{t}{t^2-1} \\
    t y & = & \int \frac{t}{t^2-1} ~ dt.
  \end{eqnarray*}

\end{frame}



\begin{frame}
  \frametitle{Partial Fractions}

  \vspace{-3em}
  \begin{eqnarray*}
    \frac{t}{(t-1)(t+1)} & = & \frac{A}{t-1} + \frac{B}{t+1} \\
    t & = & A(t+1) + B(t-1)
  \end{eqnarray*}

  Let $t=-1$
  \begin{eqnarray*}
    -1 & = & -2B, \\
    B & = & \half
  \end{eqnarray*}

  Let $t=1$
  \begin{eqnarray*}
    1 & = & 2A \\
    A & = & \half
  \end{eqnarray*}

  \begin{eqnarray*}
    t y & = & \int \frac{\half}{t-1} + \frac{\half}{t+1} ~ dt \\
    t y & = & \half \ln(t-1) + \half \ln(t+1) \\
    y &  = & \frac{\half \ln(t-1) + \half \ln(t+1)}{t}
  \end{eqnarray*}


\end{frame}


\begin{frame}
  \frametitle{Example}

  \begin{eqnarray*}
    y' & = & \cos(t) y - \cos(t) \\
    \uncover<2->{ y' & = & \cos(t) \lp y-1 \rp,} \\
    \uncover<3->{\frac{y'}{y-1} & = & \cos(t) \\
      \ln(y-1) & = & \sin(t) + C \\
      y - 1 & = & k e^{\sin(t)} \\
      y & = & 1 + ke^{\sin(t)} }
  \end{eqnarray*}

\end{frame}



% LocalWords:  Clarkson pausesection hideallsubsections
