\part{More-Undetermined-Coefficients}
\lecture{More Undetermined Coefficients}{More-Undetermined-Coefficients}
\section{More Undetermined Coefficients}

\title{Ordinary Differential Equations}
\subtitle{Math 232 - Week 8, Day 3}
\date{21 Oct 2012}

\begin{frame}
  \titlepage
\end{frame}

\begin{frame}
  \frametitle{Outline}
  \tableofcontents[pausesection,hideothersubsections]
\end{frame}


\subsection{Non-homogeneous Equations (continued)}


\begin{frame}
  \frametitle{Example}

  \begin{eqnarray*}
    y'' + 3y' + 2y & = & 4 e^{-t}.
  \end{eqnarray*}

  \uncover<2->
  {
    Homogeneous solution:
    \begin{eqnarray*}
      r^2 + 3r + 2 & = & 0, \\
      (r+2)(r+1) & = & 0, \\
      y_h & = & C_1 e^{-2t} + C_2 e^{-t}
    \end{eqnarray*}
  }

\end{frame}

\begin{frame}
  \frametitle{Particular Solution}

  \begin{eqnarray*}
    y_p & = & A t e^{-t} \\
    y_p' & = & A e^{-t} - Ate^{-t} \\
    y_p'' & = & -2A e^{-t} + At e^{-t} \\
    -2A e^{-t} + At e^{-t} + 3 \lp A e^{-t} - Ate^{-t} \rp 
    + 2 A t e^{-t} & = & 4 e^{-t}, \\
    A e^{-t} & = & 4 e^{-t} \\
    A & = & 4.
  \end{eqnarray*}

  Solution:
  \begin{eqnarray*}
    y & = & C_1 e^{-2t} + C_2 e^{-t} + 4 t e^{-t}.
  \end{eqnarray*}

\end{frame}


\begin{frame}
  \frametitle{Example}

  \begin{eqnarray*}
    y'' + 4y' + 4y & = & 5 e^{-2t}.
  \end{eqnarray*}

  \uncover<2->
  {
    Homogeneous solution:
    \begin{eqnarray*}
      r^2 + 4r + 4 & = & 0, \\
      (r+2)^2 & = & 0, \\
      y_h & = & C_1 e^{-2t} + C_2 t e^{-2t}
    \end{eqnarray*}
  }

\end{frame}

\begin{frame}
  \frametitle{Particular Solution}

  \begin{eqnarray*}
    y_p & = & A t^2 e^{-2t} \\
    y_p' & = & -2 A t^2 e^{-2t} + A 2t e^{-2t} \\
    y_p'' & = & 4 A t^2 e^{-2t} - 8A t e^{-2t} + 2 A e^{-2t} \\
    4 A t^2 e^{-2t} - 8A t e^{-2t} + 2 A e^{-2t} & & \\
    + 4 \lp -2 A t^2 e^{-2t} + A 2t e^{-2t} \rp & & \\
    + 4 A t^2 e^{-2t} & = & 5 e^{-2t} \\
    2 A e^{-2t} & = & 5 e^{-2t} \\
    A & = & \frac{5}{2}.
  \end{eqnarray*}

  Solution:
  \begin{eqnarray*}
    y & = & C_1 e^{-2t} + C_2 t e^{-2 t} + \frac{5}{2} t^2 e^{-2t}.
  \end{eqnarray*}

\end{frame}

\subsection{Cauchy-Euler Equations}

\begin{frame}
  \frametitle{Cauchy-Euler Equations}

  \begin{eqnarray*}
    a t^2 y'' + b t y' + c y & = & 0.
  \end{eqnarray*}

  \uncover<2->
  {
    Assume that the solution is in the form of
    \begin{eqnarray*}
      y & = & A t^r.
    \end{eqnarray*}
  }

\end{frame}


\begin{frame}
  \frametitle{Cauchy-Euler Equations}

  Assume that the solution is in the form of
  \begin{eqnarray*}
    y & = & A t^r \\
    y' & = & A r t^{r-1} \\
    y'' & = & A r (r-1) t^{r-2}
  \end{eqnarray*}

  Substitute back into the equation to get
  \begin{eqnarray*}
    a t^2 A r (r-1) t^{r-2} + b t A r t^{r-1} + c A t^r & = & 0, \\
    a A r (r-1) t^{r} + b A r t^{r} + c A t^r & = & 0,  \\
    A t^r \lp a r (r-1) + br + c \rp & = & 0, \\
    a r (r-1) + br + c & = & 0.
  \end{eqnarray*}

  The solution is of the form
  \begin{eqnarray*}
    y & = & C_1 t^{r_1} + C_2 t^{r_2}.
  \end{eqnarray*}
  

\end{frame}


\begin{frame}
  \frametitle{Example}

  \begin{eqnarray*}
    t^2 y'' + t y' - 3t & = & 0.
  \end{eqnarray*}

  Assume that the solution is in the form of $y=At^r$:
  \begin{eqnarray*}
    r(r-1) + r - 3 & = & 0, \\
    r^2 - 3 & = & 0, \\
    r & = & \pm \sqrt{3}.
  \end{eqnarray*}

  The solution is 
  \begin{eqnarray*}
    y & = & C_1 t^{\sqrt{3}} + C_2 t^{-\sqrt{3}}.
  \end{eqnarray*}

\end{frame}


\begin{frame}
  \frametitle{Example}


  \begin{eqnarray*}
    t y'' - 4 y' + 3 \frac{y}{t} & = & 0, \\
    \uncover<2->
    {
      t^2 y'' - 4t y' + 3y & = & 0
    }
  \end{eqnarray*}

  \uncover<3->
  {
    Assume that the solution is in the form of $y=At^r$:
  \begin{eqnarray*}
    r(r-1) - 4r + 3 & = & 0, \\
    r^2 - 5r - 3 & = & 0, \\
    r & = & \frac{5 \pm \sqrt{13}}{2}
  \end{eqnarray*}

  The solution is 
  \begin{eqnarray*}
    y & = & C_1 t^{\frac{5 + \sqrt{13}}{2}} + C_2 t^{\frac{5 - \sqrt{13}}{2}}.
  \end{eqnarray*}


  }

\end{frame}


\subsection{Reduction of Order}

\begin{frame}
  \frametitle{Reduction of Order}

  Suppose that $y_1(t)$ is \textbf{a} solution to the homogeneous part
  of
  \begin{eqnarray*}
    a y'' + by' + cy & = & f(t).
  \end{eqnarray*}

  \uncover<2->
  {
    Let
    \begin{eqnarray*}
      y_p & = & u(t) y_1(t), \\
      y_p' & = & u'(t) y_1(t) + u(t) y_1'(t) \\
      y_p'' & = & u''(t) y_1(t) + 2 u'(t) y_1'(t) + u(t) y_1''(t)
    \end{eqnarray*}
  }

\end{frame}


\begin{frame}
  \frametitle{Substitute this back into the original equation}

  \begin{eqnarray*}
    a \lp u''(t) y_1(t) + 2 u'(t) y_1'(t) + u(t) y_1''(t) \rp & & \\
    + b \lp u'(t) y_1(t) + u(t) y_1'(t) \rp & & \\
    c u(t) y_1(t) & = & f(t) 
  \end{eqnarray*}

  \begin{eqnarray*}
    \begin{array}{r|r|cl}
      \cline{2-2}
      a u''(t) y_1(t) + 2 a u'(t) y_1'(t) + & a u(t) y_1''(t)  & & \\ 
      + b  u'(t) y_1(t) + & b u(t) y_1'(t)  & & \\
      & c u(t) y_1(t) & = & f(t)  \\       \cline{2-2}
    \end{array}
  \end{eqnarray*}

\end{frame}


\begin{frame}
  \frametitle{Reduction of Order}

  The equation reduces to
  \begin{eqnarray*}
    a u''(t) y_1(t) + 2 a u'(t) y_1'(t) + b  u'(t) y_1(t) & = & f(t).
  \end{eqnarray*}

  Let $v=u'$ so the equation is now
  \begin{eqnarray*}
    a v' y_1 + 2 a v y_1' + b v y_1 & = & f(t).
  \end{eqnarray*}
  This is a first order, linear equation! We can solve this!


\end{frame}


\begin{frame}
  \frametitle{Example}

  \begin{eqnarray*}
    y'' + 2 y' + y & = & 2 e^{-t}.
  \end{eqnarray*}

  The homogeneous solution satisfies
  \begin{eqnarray*}
    r^2 + 2r + 1 & = & 0, \\
    (r+1)^2 & = & 0, \\
    r & = & -1.
  \end{eqnarray*}

  The homogeneous solution is
  \begin{eqnarray*}
    y_h & = & C_1 e^{-t} + C_2 t e^{-t}.
  \end{eqnarray*}

\end{frame}


\begin{frame}
  \frametitle{Reduction of Order}

  Let 
  \begin{eqnarray*}
    y & = & u e^{-t}.
  \end{eqnarray*}

  Take the derivatives
  \begin{eqnarray*}
    y' & = & u' e^{-t} - u e^{-t} \\
    y'' & = & u'' e^{-t} - 2 u' e^{-t} + u e^{-t}
  \end{eqnarray*}

  Substitute back into the original equation:
  \begin{eqnarray*}
    u'' e^{-t} - 2 u' e^{-t} + u e^{-t} + 2 u' e^{-t} - 2ue^{-t} + u e^{-t} & = & 2 e^{-t}    \\
    u'' e^{-t} & = & 2 e^{-t} \\
    u'' & = & 2.
  \end{eqnarray*}

\end{frame}

\begin{frame}

  Solving this differential equation we get
  \begin{eqnarray*}
    u & = & t^2 + C_1 t + C_2, \\
    y & = & \lp  t^2 + C_1 t + C_2 \rp e^{-t}
  \end{eqnarray*}
  
\end{frame}



% LocalWords:  Clarkson pausesection hideothersubsections
